src/lib/Lens.v
@@ -1,0 +1,69 @@
+From Coq Require Import Program.
+
+Module Store.
+
+  Definition t S A := (S * (S -> A))%type.
+
+  Definition map {S A B} : (A -> B) -> t S A -> t S B :=
+    fun ϕ '(a, f) => (a, ϕ ∘ f).
+
+  Definition counit {S A} : t S A -> A :=
+    fun '(a, f) => f a.
+
+  Definition cojoin {S A} : t S A -> t S (t S A) :=
+    fun '(a, f) => (a, fun a' => (a', f)).
+
+End Store.
+
+Module Lens.
+
+  Definition t S V := S -> Store.t V S.
+  Definition view {S V} : t S V -> S -> V := fun l s => fst (l s).
+  Definition set {S V} : t S V -> V -> S -> S := fun l a s => snd (l s) a.
+
+  (* Lens is just a coalgebra of the Store comonad *)
+  Record isLens {S V} (l : t S V) : Prop :=
+    { counit : Store.counit ∘ l = id
+    ; coaction : Store.map l ∘ l = Store.cojoin ∘ l
+    }.
+
+  Definition compose {A B C} : t A B -> t B C -> t A C.
+  Proof.
+    intros l1 l2.
+    intro a. split.
+    - exact (view l2 (view l1 a)).
+    - intro c. exact (set l1 (set l2 c (view l1 a)) a).
+  Defined.
+
+  Lemma compose_assoc A B C D (l1 : t A B) (l2 : t B C) (l3 : t C D) :
+    (compose (compose l1 l2) l3) = compose l1 (compose l2 l3).
+  Proof. reflexivity. Qed.
+
+End Lens.
+
+Declare Scope lens_scope.
+Delimit Scope lens_scope with lens.
+Infix "⋅" := (Lens.compose) (at level 50, left associativity) : lens_scope.
+
+Section PRODUCT_LENS.
+
+  Context {A B : Type}.
+
+  Definition fstl : Lens.t (A * B) A := fun '(a, b) => (a, fun a' => (a', b)).
+  Definition sndl : Lens.t (A * B) B := fun '(a, b) => (b, fun b' => (a, b')).
+
+End PRODUCT_LENS.
+
+Section TEST.
+
+  Let lens1 : Lens.t ((nat * nat) * nat) nat := (fstl ⋅ fstl)%lens.
+  Let lens2 : Lens.t ((nat * nat) * nat) nat := (fstl ⋅ sndl)%lens.
+  Let lens3 : Lens.t ((nat * nat) * nat) nat := sndl.
+  Goal Lens.view lens1 (1,2,3) = 1. reflexivity. Qed.
+  Goal Lens.view lens2 (1,2,3) = 2. reflexivity. Qed.
+  Goal Lens.view lens3 (1,2,3) = 3. reflexivity. Qed.
+  Goal Lens.set lens1 4 (1,2,3) = (4,2,3). reflexivity. Qed.
+  Goal Lens.set lens2 4 (1,2,3) = (1,4,3). reflexivity. Qed.
+  Goal Lens.set lens3 4 (1,2,3) = (1,2,4). reflexivity. Qed.
+
+End TEST.
