src/semantics/Wrapper.v
@@ -56,7 +56,7 @@ Module WMod.
         _ <- trigger Yield;;
 
         tid <- trigger (GetTid);;
-        '(st, ts) <- trigger (@Get _);;
+        '(st, ts) <- trigger (Get id);;
         let ts := NatMap.add tid f.(type) ts in
         _ <- trigger (Put (st, ts));;
         _ <- trigger (Fair (sum_fmap_l (fun i => if tid_dec i tid then Flag.success else Flag.emp)));;
@@ -69,7 +69,7 @@ Module WMod.
                _ <- trigger (Fair (sum_fmap_l (fun i => if tid_dec i tid then Flag.fail else Flag.emp)));;
                _ <- trigger Yield;; Ret (inl tt)
              else
-               '(st, ts) <- trigger (@Get _);;
+               '(st, ts) <- trigger (Get id);;
                next <- trigger (Choose (sig (f.(body) arg st)));;
                match proj1_sig next with
                | normal st r fm =>
@@ -84,7 +84,7 @@ Module WMod.
     .
 
     Definition interp_fun_register (tid: thread_id) (i: m.(ident)): itree (programE interp_ident interp_state) unit :=
-      '(st, ts) <- trigger (@Get _);;
+      '(st, ts) <- trigger (Get id);;
       let ts := NatMap.add tid i ts in
       _ <- trigger (Put (st, ts));;
       _ <- trigger (Fair (sum_fmap_l (fun i => if tid_dec i tid then Flag.success else Flag.emp)));;
@@ -101,7 +101,7 @@ Module WMod.
              _ <- trigger (Fair (sum_fmap_l (fun i => if tid_dec i tid then Flag.fail else Flag.emp)));;
              _ <- trigger Yield;; Ret (inl tt)
            else
-             '(st, ts) <- trigger (@Get _);;
+             '(st, ts) <- trigger (Get id);;
              next <- trigger (Choose (sig (step st)));;
              match proj1_sig next with
              | normal st r fm =>
@@ -139,7 +139,7 @@ Module WMod.
           _ <- trigger Yield;;
           tau;; interp_fun_body tid step
         else
-          '(st, ts) <- trigger (@Get _);;
+          '(st, ts) <- trigger (Get id);;
           next <- trigger (Choose (sig (step st)));;
           match proj1_sig next with
           | normal st r fm =>
