src/simulation/ModSim.v
@@ -68,20 +68,13 @@ Section PRIMIVIESIM.
       (LSIM: exists x, _lsim _ _ RR true f_tgt r_ctx (ktr_src x) itr_tgt (ths, im_src, im_tgt, st_src, st_tgt))
     :
     __lsim tid lsim _lsim RR f_src f_tgt r_ctx (trigger (Choose X) >>= ktr_src) itr_tgt (ths, im_src, im_tgt, st_src, st_tgt)
-  | lsim_putL
+  | lsim_rmwL
       f_src f_tgt r_ctx
       ths im_src im_tgt st_src st_tgt
-      st ktr_src itr_tgt
-      (LSIM: _lsim _ _ RR true f_tgt r_ctx (ktr_src tt) itr_tgt (ths, im_src, im_tgt, st, st_tgt))
+      X rmw ktr_src itr_tgt
+      (LSIM: _lsim _ _ RR true f_tgt r_ctx (ktr_src (snd (rmw st_src) : X)) itr_tgt (ths, im_src, im_tgt, fst (rmw st_src), st_tgt))
     :
-    __lsim tid lsim _lsim RR f_src f_tgt r_ctx (trigger (Put st) >>= ktr_src) itr_tgt (ths, im_src, im_tgt, st_src, st_tgt)
-  | lsim_getL
-      f_src f_tgt r_ctx
-      ths im_src im_tgt st_src st_tgt
-      ktr_src itr_tgt
-      (LSIM: _lsim _ _ RR true f_tgt r_ctx (ktr_src st_src) itr_tgt (ths, im_src, im_tgt, st_src, st_tgt))
-    :
-    __lsim tid lsim _lsim RR f_src f_tgt r_ctx (trigger (@Get _) >>= ktr_src) itr_tgt (ths, im_src, im_tgt, st_src, st_tgt)
+    __lsim tid lsim _lsim RR f_src f_tgt r_ctx (trigger (Rmw rmw) >>= ktr_src) itr_tgt (ths, im_src, im_tgt, st_src, st_tgt)
   | lsim_tidL
       f_src f_tgt r_ctx
       ths im_src im_tgt st_src st_tgt
@@ -119,20 +112,13 @@ Section PRIMIVIESIM.
       (LSIM: forall x, _lsim _ _ RR f_src true r_ctx itr_src (ktr_tgt x) (ths, im_src, im_tgt, st_src, st_tgt))
     :
     __lsim tid lsim _lsim RR f_src f_tgt r_ctx itr_src (trigger (Choose X) >>= ktr_tgt) (ths, im_src, im_tgt, st_src, st_tgt)
-  | lsim_putR
+  | lsim_rmwR
       f_src f_tgt r_ctx
       ths im_src im_tgt st_src st_tgt
-      st itr_src ktr_tgt
-      (LSIM: _lsim _ _ RR f_src true r_ctx itr_src (ktr_tgt tt) (ths, im_src, im_tgt, st_src, st))
+      X rmw itr_src ktr_tgt
+      (LSIM: _lsim _ _ RR f_src true r_ctx itr_src (ktr_tgt (snd (rmw st_tgt) : X)) (ths, im_src, im_tgt, st_src, fst (rmw st_tgt)))
     :
-    __lsim tid lsim _lsim RR f_src f_tgt r_ctx itr_src (trigger (Put st) >>= ktr_tgt) (ths, im_src, im_tgt, st_src, st_tgt)
-  | lsim_getR
-      f_src f_tgt r_ctx
-      ths im_src im_tgt st_src st_tgt
-      itr_src ktr_tgt
-      (LSIM: _lsim _ _ RR f_src true r_ctx itr_src (ktr_tgt st_tgt) (ths, im_src, im_tgt, st_src, st_tgt))
-    :
-    __lsim tid lsim _lsim RR f_src f_tgt r_ctx itr_src (trigger (@Get _) >>= ktr_tgt) (ths, im_src, im_tgt, st_src, st_tgt)
+    __lsim tid lsim _lsim RR f_src f_tgt r_ctx itr_src (trigger (Rmw rmw) >>= ktr_tgt) (ths, im_src, im_tgt, st_src, st_tgt)
   | lsim_tidR
       f_src f_tgt r_ctx
       ths im_src im_tgt st_src st_tgt
@@ -334,11 +320,7 @@ Section PRIMIVIESIM.
       destruct LSIM0 as [LSIM0 IND]. hexploit IH; eauto.
     }
 
-    { eapply pind9_fold. eapply lsim_putL. split; ss.
-      destruct LSIM0 as [LSIM0 IND]. hexploit IH; eauto.
-    }
-
-    { eapply pind9_fold. eapply lsim_getL. split; ss.
+    { eapply pind9_fold. eapply lsim_rmwL. split; ss.
       destruct LSIM0 as [LSIM0 IND]. hexploit IH; eauto.
     }
 
@@ -361,11 +343,7 @@ Section PRIMIVIESIM.
       destruct LSIM0 as [LSIM0 IND]. hexploit IH; eauto.
     }
 
-    { eapply pind9_fold. eapply lsim_putR. split; ss.
-      destruct LSIM0 as [LSIM0 IND]. hexploit IH; eauto.
-    }
-
-    { eapply pind9_fold. eapply lsim_getR. split; ss.
+    { eapply pind9_fold. eapply lsim_rmwR. split; ss.
       destruct LSIM0 as [LSIM0 IND]. hexploit IH; eauto.
     }
 
@@ -457,11 +435,7 @@ Section PRIMIVIESIM.
       destruct LSIM0 as [LSIM0 IND]. hexploit IH; eauto.
     }
 
-    { eapply pind9_fold. eapply lsim_putL. split; ss.
-      destruct LSIM0 as [LSIM0 IND]. hexploit IH; eauto.
-    }
-
-    { eapply pind9_fold. eapply lsim_getL. split; ss.
+    { eapply pind9_fold. eapply lsim_rmwL. split; ss.
       destruct LSIM0 as [LSIM0 IND]. hexploit IH; eauto.
     }
 
@@ -484,11 +458,7 @@ Section PRIMIVIESIM.
       destruct LSIM0 as [LSIM0 IND]. hexploit IH; eauto.
     }
 
-    { eapply pind9_fold. eapply lsim_putR. split; ss.
-      destruct LSIM0 as [LSIM0 IND]. hexploit IH; eauto.
-    }
-
-    { eapply pind9_fold. eapply lsim_getR. split; ss.
+    { eapply pind9_fold. eapply lsim_rmwR. split; ss.
       destruct LSIM0 as [LSIM0 IND]. hexploit IH; eauto.
     }
 
@@ -577,11 +547,7 @@ Section PRIMIVIESIM.
       destruct LSIM0 as [LSIM0 IND]. hexploit IH; eauto.
     }
 
-    { guclo lsim_indC_spec. eapply lsim_putL.
-      destruct LSIM0 as [LSIM0 IND]. hexploit IH; eauto.
-    }
-
-    { guclo lsim_indC_spec. eapply lsim_getL.
+    { guclo lsim_indC_spec. eapply lsim_rmwL.
       destruct LSIM0 as [LSIM0 IND]. hexploit IH; eauto.
     }
 
@@ -604,11 +570,7 @@ Section PRIMIVIESIM.
       destruct LSIM0 as [LSIM0 IND]. hexploit IH; eauto.
     }
 
-    { guclo lsim_indC_spec. eapply lsim_putR.
-      destruct LSIM0 as [LSIM0 IND]. hexploit IH; eauto.
-    }
-
-    { guclo lsim_indC_spec. eapply lsim_getR.
+    { guclo lsim_indC_spec. eapply lsim_rmwR.
       destruct LSIM0 as [LSIM0 IND]. hexploit IH; eauto.
     }
 
@@ -726,11 +688,7 @@ Section PRIMIVIESIM.
       destruct LSIM0 as [LSIM0 IND]. hexploit IH; eauto.
     }
 
-    { guclo lsim_indC_spec. eapply lsim_putL.
-      destruct LSIM0 as [LSIM0 IND]. hexploit IH; eauto.
-    }
-
-    { guclo lsim_indC_spec. eapply lsim_getL.
+    { guclo lsim_indC_spec. eapply lsim_rmwL.
       destruct LSIM0 as [LSIM0 IND]. hexploit IH; eauto.
     }
 
@@ -753,11 +711,7 @@ Section PRIMIVIESIM.
       destruct LSIM0 as [LSIM0 IND]. hexploit IH; eauto.
     }
 
-    { guclo lsim_indC_spec. eapply lsim_putR.
-      destruct LSIM0 as [LSIM0 IND]. hexploit IH; eauto.
-    }
-
-    { guclo lsim_indC_spec. eapply lsim_getR.
+    { guclo lsim_indC_spec. eapply lsim_rmwR.
       destruct LSIM0 as [LSIM0 IND]. hexploit IH; eauto.
     }
 
@@ -858,11 +812,7 @@ Section PRIMIVIESIM.
       destruct LSIM0 as [LSIM0 IND]. hexploit IH; eauto. i. punfold H.
     }
 
-    { pfold. eapply pind9_fold. eapply lsim_putL. split; ss.
-      destruct LSIM0 as [LSIM0 IND]. hexploit IH; eauto. i. punfold H.
-    }
-
-    { pfold. eapply pind9_fold. eapply lsim_getL. split; ss.
+    { pfold. eapply pind9_fold. eapply lsim_rmwL. split; ss.
       destruct LSIM0 as [LSIM0 IND]. hexploit IH; eauto. i. punfold H.
     }
 
@@ -885,11 +835,7 @@ Section PRIMIVIESIM.
       destruct LSIM0 as [LSIM0 IND]. hexploit IH; eauto. i. punfold H.
     }
 
-    { pfold. eapply pind9_fold. eapply lsim_putR. split; ss.
-      destruct LSIM0 as [LSIM0 IND]. hexploit IH; eauto. i. punfold H.
-    }
-
-    { pfold. eapply pind9_fold. eapply lsim_getR. split; ss.
+    { pfold. eapply pind9_fold. eapply lsim_rmwR. split; ss.
       destruct LSIM0 as [LSIM0 IND]. hexploit IH; eauto. i. punfold H.
     }
 
@@ -1020,8 +966,6 @@ Section PRIMIVIESIM.
     { eapply f_equal with (f:=observe) in H3. ss. }
     { eapply f_equal with (f:=observe) in H3. ss. }
     { eapply f_equal with (f:=observe) in H3. ss. }
-    { eapply f_equal with (f:=observe) in H3. ss. }
-    { eapply f_equal with (f:=observe) in H4. ss. }
     { eapply f_equal with (f:=observe) in H4. ss. }
     { eapply f_equal with (f:=observe) in H4. ss. }
     { eapply f_equal with (f:=observe) in H4. ss. }
@@ -1054,9 +998,7 @@ Section PRIMIVIESIM.
     { eapply f_equal with (f:=observe) in H3. ss. }
     { eapply f_equal with (f:=observe) in H3. ss. }
     { eapply f_equal with (f:=observe) in H3. ss. }
-    { eapply f_equal with (f:=observe) in H3. ss. }
     { inv LSIM0. eapply lsim_flag_any. pfold. eauto. }
-    { eapply f_equal with (f:=observe) in H4. ss. }
     { eapply f_equal with (f:=observe) in H4. ss. }
     { eapply f_equal with (f:=observe) in H4. ss. }
     { eapply f_equal with (f:=observe) in H4. ss. }
@@ -1090,12 +1032,10 @@ Section PRIMIVIESIM.
     { eapply f_equal with (f:=observe) in H3. ss. }
     { eapply f_equal with (f:=observe) in H3. ss. }
     { eapply f_equal with (f:=observe) in H3. ss. }
-    { eapply f_equal with (f:=observe) in H3. ss. }
     { eapply f_equal with (f:=observe) in H4. ss. }
     { eapply trigger_eq_rev in H4. des. subst.
       i. specialize (LSIM0 x). inv LSIM0.
       eapply lsim_flag_any. pfold. eauto. }
-    { eapply trigger_eq_rev in H4. des. subst. dependent destruction H0. }
     { eapply trigger_eq_rev in H4. des. subst. dependent destruction H0. }
     { eapply trigger_eq_rev in H4. des. subst. dependent destruction H0. }
     { eapply trigger_eq_rev in H4. des. subst. dependent destruction H0. }
@@ -1145,8 +1085,6 @@ Section PRIMIVIESIM.
     { eapply f_equal with (f:=observe) in H3. ss. }
     { eapply f_equal with (f:=observe) in H3. ss. }
     { eapply f_equal with (f:=observe) in H3. ss. }
-    { eapply f_equal with (f:=observe) in H3. ss. }
-    { eapply f_equal with (f:=observe) in H4. ss. }
     { eapply f_equal with (f:=observe) in H4. ss. }
     { eapply f_equal with (f:=observe) in H4. ss. }
     { eapply f_equal with (f:=observe) in H4. ss. }
@@ -1182,8 +1120,6 @@ Section PRIMIVIESIM.
     { eapply f_equal with (f:=observe) in H3. ss. }
     { eapply f_equal with (f:=observe) in H3. ss. }
     { eapply f_equal with (f:=observe) in H3. ss. }
-    { eapply f_equal with (f:=observe) in H3. ss. }
-    { eapply f_equal with (f:=observe) in H4. ss. }
     { eapply f_equal with (f:=observe) in H4. ss. }
     { eapply f_equal with (f:=observe) in H4. ss. }
     { eapply trigger_eq_rev in H4. des. exfalso.
@@ -1220,119 +1156,12 @@ Section PRIMIVIESIM.
     { eapply f_equal with (f:=observe) in H3. ss. }
     { eapply f_equal with (f:=observe) in H3. ss. }
     { eapply f_equal with (f:=observe) in H3. ss. }
-    { eapply f_equal with (f:=observe) in H3. ss. }
     { eapply f_equal with (f:=observe) in H4. ss. }
-    { eapply trigger_eq_rev in H4. des. subst. dependent destruction H0. }
-    { eapply trigger_eq_rev in H4. des. dependent destruction H0. }
-    { eapply trigger_eq_rev in H4. des. exfalso.
-      clear - H4 H0 H1. subst. dependent destruction H0.
-    }
-    { eapply trigger_eq_rev in H4. des. exfalso.
-      eapply nat_not_unit; eauto.
-    }
-    { eapply trigger_eq_rev in H4. des. dependent destruction H0. }
-    { eapply trigger_eq_rev in H4. des. exfalso.
-      eapply nat_not_unit; eauto.
-    }
-    { eapply f_equal with (f:=observe) in H3. ss. }
-    { eapply f_equal with (f:=observe) in H3. ss. }
-    { eapply f_equal with (f:=observe) in H3. ss. }
-    { eapply f_equal with (f:=observe) in H3. ss. }
-  Qed.
-
-  Lemma lsim_rev_get
-        tid
-        R0 R1 (RR: R0 -> R1 -> URA.car -> shared_rel)
-        r_src tgt ths im_src im_tgt st_src st_tgt ps pt r_ctx
-        (LSIM: lsim tid RR ps pt r_ctx (Ret r_src) (trigger (@Get _) >>= tgt) (ths, im_src, im_tgt, st_src, st_tgt))
-    :
-    lsim tid RR ps pt r_ctx (Ret r_src) (tgt st_tgt) (ths, im_src, im_tgt, st_src, st_tgt).
-  Proof.
-    eapply lsim_reset_prog in LSIM.
-    2:{ i. reflexivity. }
-    2:{ i. reflexivity. }
-    eapply lsim_set_prog in LSIM.
-    instantiate (1:=false) in LSIM. instantiate (1:=false) in LSIM.
-    punfold LSIM. eapply pind9_unfold in LSIM; auto.
-    2:{ eapply _lsim_mon. }
-    inv LSIM; auto.
+    { eapply f_equal with (f:=observe) in H4. ss. }
+    { eapply f_equal with (f:=observe) in H4. ss. }
+    { eapply f_equal with (f:=observe) in H4. ss. }
     { eapply f_equal with (f:=observe) in H4. ss. }
     { eapply f_equal with (f:=observe) in H3. ss. }
-    { eapply f_equal with (f:=observe) in H3. ss. }
-    { eapply f_equal with (f:=observe) in H3. ss. }
-    { eapply f_equal with (f:=observe) in H3. ss. }
-    { eapply f_equal with (f:=observe) in H3. ss. }
-    { eapply f_equal with (f:=observe) in H3. ss. }
-    { eapply f_equal with (f:=observe) in H4. ss. }
-    { eapply trigger_eq_rev in H4. des. subst. dependent destruction H0. }
-    { eapply trigger_eq_rev in H4. des. exfalso.
-      clear - H4 H0 H1. subst. dependent destruction H0.
-    }
-    { eapply trigger_eq_rev in H4. des. subst.
-      inv LSIM0. eapply lsim_flag_any. pfold. eauto.
-    }
-    { eapply trigger_eq_rev in H4. des. exfalso.
-      clear - H4 H0 H1. subst. dependent destruction H0.
-    }
-    { eapply trigger_eq_rev in H4. des. exfalso.
-      clear - H4 H0 H1. subst. dependent destruction H0.
-    }
-    { eapply trigger_eq_rev in H4. des. exfalso.
-      clear - H4 H0 H1. subst. dependent destruction H0.
-    }
-    { eapply trigger_eq_rev in H4. des. exfalso.
-      clear - H4 H0 H1. subst. dependent destruction H0.
-    }
-    { eapply trigger_eq_rev in H4. des. exfalso.
-      clear - H4 H0 H1. subst. dependent destruction H0.
-    }
-    { eapply trigger_eq_rev in H4. des. exfalso.
-      clear - H4 H0 H1. subst. dependent destruction H0.
-    }
-    { eapply f_equal with (f:=observe) in H3. ss. }
-  Qed.
-
-  Lemma lsim_rev_put
-        tid
-        R0 R1 (RR: R0 -> R1 -> URA.car -> shared_rel)
-        r_src tgt ths im_src im_tgt st_src st_tgt ps pt r_ctx
-        st
-        (LSIM: lsim tid RR ps pt r_ctx (Ret r_src) (trigger (Put st) >>= tgt) (ths, im_src, im_tgt, st_src, st_tgt))
-    :
-    lsim tid RR ps pt r_ctx (Ret r_src) (tgt tt) (ths, im_src, im_tgt, st_src, st).
-  Proof.
-    eapply lsim_reset_prog in LSIM.
-    2:{ i. reflexivity. }
-    2:{ i. reflexivity. }
-    eapply lsim_set_prog in LSIM.
-    instantiate (1:=false) in LSIM. instantiate (1:=false) in LSIM.
-    punfold LSIM. eapply pind9_unfold in LSIM; auto.
-    2:{ eapply _lsim_mon. }
-    inv LSIM; auto.
-    { eapply f_equal with (f:=observe) in H4. ss. }
-    { eapply f_equal with (f:=observe) in H3. ss. }
-    { eapply f_equal with (f:=observe) in H3. ss. }
-    { eapply f_equal with (f:=observe) in H3. ss. }
-    { eapply f_equal with (f:=observe) in H3. ss. }
-    { eapply f_equal with (f:=observe) in H3. ss. }
-    { eapply f_equal with (f:=observe) in H3. ss. }
-    { eapply f_equal with (f:=observe) in H4. ss. }
-    { eapply trigger_eq_rev in H4. des. subst. dependent destruction H0. }
-    { eapply trigger_eq_rev in H4. des. subst. dependent destruction H0.
-      inv LSIM0. eapply lsim_flag_any. pfold. eauto.
-    }
-    { eapply trigger_eq_rev in H4. des. exfalso.
-      clear - H4 H0 H1. subst. dependent destruction H0.
-    }
-    { eapply trigger_eq_rev in H4. des. exfalso.
-      eapply nat_not_unit; ss.
-    }
-    { eapply trigger_eq_rev in H4. des. exfalso.
-      clear - H4 H0 H1. subst. dependent destruction H0.
-    }
-    { eapply trigger_eq_rev in H4. des. exfalso.
-      eapply nat_not_unit; eauto.
-    }
     { eapply f_equal with (f:=observe) in H3. ss. }
     { eapply f_equal with (f:=observe) in H3. ss. }
     { eapply f_equal with (f:=observe) in H3. ss. }
@@ -1364,13 +1193,9 @@ Section PRIMIVIESIM.
     { eapply f_equal with (f:=observe) in H3. ss. }
     { eapply f_equal with (f:=observe) in H3. ss. }
     { eapply f_equal with (f:=observe) in H3. ss. }
-    { eapply f_equal with (f:=observe) in H3. ss. }
     { eapply f_equal with (f:=observe) in H4. ss. }
     { eapply trigger_eq_rev in H4. des. subst. dependent destruction H0. }
     { eapply trigger_eq_rev in H4. des. subst. dependent destruction H0. }
-    { eapply trigger_eq_rev in H4. des. exfalso.
-      clear - H4 H0 H1. subst. dependent destruction H0.
-    }
     { eapply trigger_eq_rev in H4. des. exfalso.
       eapply nat_not_unit; ss.
     }
