src/simulation/ModSimYOrd.v
@@ -70,20 +70,13 @@ Section PRIMIVIESIM.
       (LSIM: exists x, _lsim _ _ RR true f_tgt r_ctx (os, ktr_src x) (ot, itr_tgt) (ths, im_src, im_tgt, st_src, st_tgt))
     :
     __lsim tid lsim _lsim RR f_src f_tgt r_ctx (os, trigger (Choose X) >>= ktr_src) (ot, itr_tgt) (ths, im_src, im_tgt, st_src, st_tgt)
-  | lsim_putL
+  | lsim_rmwL
       f_src f_tgt r_ctx os ot
       ths im_src im_tgt st_src st_tgt
-      st ktr_src itr_tgt
-      (LSIM: _lsim _ _ RR true f_tgt r_ctx (os, ktr_src tt) (ot, itr_tgt) (ths, im_src, im_tgt, st, st_tgt))
+      X rmw ktr_src itr_tgt
+      (LSIM: _lsim _ _ RR true f_tgt r_ctx (os, ktr_src (snd (rmw st_src) : X)) (ot, itr_tgt) (ths, im_src, im_tgt, fst (rmw st_src), st_tgt))
     :
-    __lsim tid lsim _lsim RR f_src f_tgt r_ctx (os, trigger (Put st) >>= ktr_src) (ot, itr_tgt) (ths, im_src, im_tgt, st_src, st_tgt)
-  | lsim_getL
-      f_src f_tgt r_ctx os ot
-      ths im_src im_tgt st_src st_tgt
-      ktr_src itr_tgt
-      (LSIM: _lsim _ _ RR true f_tgt r_ctx (os, ktr_src st_src) (ot, itr_tgt) (ths, im_src, im_tgt, st_src, st_tgt))
-    :
-    __lsim tid lsim _lsim RR f_src f_tgt r_ctx (os, trigger (@Get _) >>= ktr_src) (ot, itr_tgt) (ths, im_src, im_tgt, st_src, st_tgt)
+    __lsim tid lsim _lsim RR f_src f_tgt r_ctx (os, trigger (Rmw rmw) >>= ktr_src) (ot, itr_tgt) (ths, im_src, im_tgt, st_src, st_tgt)
   | lsim_tidL
       f_src f_tgt r_ctx os ot
       ths im_src im_tgt st_src st_tgt
@@ -121,20 +114,13 @@ Section PRIMIVIESIM.
       (LSIM: forall x, _lsim _ _ RR f_src true r_ctx (os, itr_src) (ot, ktr_tgt x) (ths, im_src, im_tgt, st_src, st_tgt))
     :
     __lsim tid lsim _lsim RR f_src f_tgt r_ctx (os, itr_src) (ot, trigger (Choose X) >>= ktr_tgt) (ths, im_src, im_tgt, st_src, st_tgt)
-  | lsim_putR
+  | lsim_rmwR
       f_src f_tgt r_ctx os ot
       ths im_src im_tgt st_src st_tgt
-      st itr_src ktr_tgt
-      (LSIM: _lsim _ _ RR f_src true r_ctx (os, itr_src) (ot, ktr_tgt tt) (ths, im_src, im_tgt, st_src, st))
+      X rmw itr_src ktr_tgt
+      (LSIM: _lsim _ _ RR f_src true r_ctx (os, itr_src) (ot, ktr_tgt (snd (rmw st_tgt) : X)) (ths, im_src, im_tgt, st_src, fst (rmw st_tgt)))
     :
-    __lsim tid lsim _lsim RR f_src f_tgt r_ctx (os, itr_src) (ot, trigger (Put st) >>= ktr_tgt) (ths, im_src, im_tgt, st_src, st_tgt)
-  | lsim_getR
-      f_src f_tgt r_ctx os ot
-      ths im_src im_tgt st_src st_tgt
-      itr_src ktr_tgt
-      (LSIM: _lsim _ _ RR f_src true r_ctx (os, itr_src) (ot, ktr_tgt st_tgt) (ths, im_src, im_tgt, st_src, st_tgt))
-    :
-    __lsim tid lsim _lsim RR f_src f_tgt r_ctx (os, itr_src) (ot, trigger (@Get _) >>= ktr_tgt) (ths, im_src, im_tgt, st_src, st_tgt)
+    __lsim tid lsim _lsim RR f_src f_tgt r_ctx (os, itr_src) (ot, trigger (Rmw rmw) >>= ktr_tgt) (ths, im_src, im_tgt, st_src, st_tgt)
   | lsim_tidR
       f_src f_tgt r_ctx os ot
       ths im_src im_tgt st_src st_tgt
@@ -344,11 +330,7 @@ Section PRIMIVIESIM.
       destruct LSIM0 as [LSIM0 IND]. hexploit IH; eauto.
     }
 
-    { eapply pind9_fold. eapply lsim_putL. split; ss.
-      destruct LSIM0 as [LSIM0 IND]. hexploit IH; eauto.
-    }
-
-    { eapply pind9_fold. eapply lsim_getL. split; ss.
+    { eapply pind9_fold. eapply lsim_rmwL. split; ss.
       destruct LSIM0 as [LSIM0 IND]. hexploit IH; eauto.
     }
 
@@ -371,11 +353,7 @@ Section PRIMIVIESIM.
       destruct LSIM0 as [LSIM0 IND]. hexploit IH; eauto.
     }
 
-    { eapply pind9_fold. eapply lsim_putR. split; ss.
-      destruct LSIM0 as [LSIM0 IND]. hexploit IH; eauto.
-    }
-
-    { eapply pind9_fold. eapply lsim_getR. split; ss.
+    { eapply pind9_fold. eapply lsim_rmwR. split; ss.
       destruct LSIM0 as [LSIM0 IND]. hexploit IH; eauto.
     }
 
@@ -465,11 +443,7 @@ Section PRIMIVIESIM.
       destruct LSIM0 as [LSIM0 IND]. hexploit IH; eauto. i. punfold H.
     }
 
-    { pfold. eapply pind9_fold. eapply lsim_putL. split; ss.
-      destruct LSIM0 as [LSIM0 IND]. hexploit IH; eauto. i. punfold H.
-    }
-
-    { pfold. eapply pind9_fold. eapply lsim_getL. split; ss.
+    { pfold. eapply pind9_fold. eapply lsim_rmwL. split; ss.
       destruct LSIM0 as [LSIM0 IND]. hexploit IH; eauto. i. punfold H.
     }
 
@@ -492,11 +466,7 @@ Section PRIMIVIESIM.
       destruct LSIM0 as [LSIM0 IND]. hexploit IH; eauto. i. punfold H.
     }
 
-    { pfold. eapply pind9_fold. eapply lsim_putR. split; ss.
-      destruct LSIM0 as [LSIM0 IND]. hexploit IH; eauto. i. punfold H.
-    }
-
-    { pfold. eapply pind9_fold. eapply lsim_getR. split; ss.
+    { pfold. eapply pind9_fold. eapply lsim_rmwR. split; ss.
       destruct LSIM0 as [LSIM0 IND]. hexploit IH; eauto. i. punfold H.
     }
 
@@ -578,11 +548,7 @@ Section PRIMIVIESIM.
       destruct LSIM0 as [LSIM0 IND]. hexploit IH; eauto.
     }
 
-    { eapply pind9_fold. eapply lsim_putL. split; ss.
-      destruct LSIM0 as [LSIM0 IND]. hexploit IH; eauto.
-    }
-
-    { eapply pind9_fold. eapply lsim_getL. split; ss.
+    { eapply pind9_fold. eapply lsim_rmwL. split; ss.
       destruct LSIM0 as [LSIM0 IND]. hexploit IH; eauto.
     }
 
@@ -605,11 +571,7 @@ Section PRIMIVIESIM.
       destruct LSIM0 as [LSIM0 IND]. hexploit IH; eauto.
     }
 
-    { eapply pind9_fold. eapply lsim_putR. split; ss.
-      destruct LSIM0 as [LSIM0 IND]. hexploit IH; eauto.
-    }
-
-    { eapply pind9_fold. eapply lsim_getR. split; ss.
+    { eapply pind9_fold. eapply lsim_rmwR. split; ss.
       destruct LSIM0 as [LSIM0 IND]. hexploit IH; eauto.
     }
 
@@ -692,11 +654,7 @@ Section PRIMIVIESIM.
       destruct LSIM0 as [LSIM0 IND]. hexploit IH; eauto.
     }
 
-    { eapply pind9_fold. eapply lsim_putL. split; ss.
-      destruct LSIM0 as [LSIM0 IND]. hexploit IH; eauto.
-    }
-
-    { eapply pind9_fold. eapply lsim_getL. split; ss.
+    { eapply pind9_fold. eapply lsim_rmwL. split; ss.
       destruct LSIM0 as [LSIM0 IND]. hexploit IH; eauto.
     }
 
@@ -719,11 +677,7 @@ Section PRIMIVIESIM.
       destruct LSIM0 as [LSIM0 IND]. hexploit IH; eauto.
     }
 
-    { eapply pind9_fold. eapply lsim_putR. split; ss.
-      destruct LSIM0 as [LSIM0 IND]. hexploit IH; eauto.
-    }
-
-    { eapply pind9_fold. eapply lsim_getR. split; ss.
+    { eapply pind9_fold. eapply lsim_rmwR. split; ss.
       destruct LSIM0 as [LSIM0 IND]. hexploit IH; eauto.
     }
 
